spc/IPM.v
@@ -178,10 +178,8 @@ Section IPM.
   Proof.
     econs.
     - ii. econs. unfold bupd. uipropall. i. split.
-      { ii. exploit H1; eauto. i. des. esplits; eauto.
-        eapply H; et. eapply URA.wf_mon; et. }
-      { ii. exploit H1; eauto. i. des. esplits; eauto.
-        eapply H; et. eapply URA.wf_mon; et. }
+      { ii. des. esplits; et. eapply H; et. eapply URA.wf_mon; et. eapply H2. rewrite URA.unit_id. et. }
+      { ii. des. esplits; et. eapply H; et. eapply URA.wf_mon; et. eapply H2. rewrite URA.unit_id. et. }
     - exact Upd_intro.
     - exact Upd_mono.
     - exact Upd_trans.
@@ -315,9 +313,7 @@ Section ILEMMAS.
       Own a ⊢ #=> P.
   Proof.
     uipropall. ss. i. unfold URA.extends in *. des. subst.
-    uipropall. i. esplits; [|apply SAT]. eapply URA.wf_mon.
-    instantiate (1:=ctx0). replace (a ⋅ ctx ⋅ ctx0) with (a ⋅ ctx0 ⋅ ctx); et.
-    repeat rewrite <- URA.add_assoc. f_equal. eapply URA.add_comm.
+    esplits; et. i. eapply (URA.wf_mon (b:=ctx)). r_wf H.
   Qed.
 
   Lemma to_semantic (a: Σ) (P: iProp') (SAT: Own a ⊢ P) (WF: URA.wf a)
@@ -339,28 +335,26 @@ Section ILEMMAS.
     :
       #=> ⌜P⌝ ⊢ ⌜P⌝.
   Proof.
-    rr. uipropall. i. rr. uipropall.
-    hexploit (H URA.unit).
-    { rewrite URA.unit_id. et. }
-    i. des. rr in H1. uipropall.
+    rr. uipropall. i. rr. uipropall. des. rr in H. uipropall.
   Qed.
 
-  Lemma Own_Upd_set
-        (r1: Σ) B
-        (UPD: URA.updatable_set r1 B)
-    :
-      (Own r1) ⊢ (#=> (∃ b, ⌜B b⌝ ** (Own b)))
-  .
-  Proof.
-    cut (Entails (Own r1) (Upd (Ex (fun b => Sepconj (Pure (B b)) (Own b))))); ss.
-    uipropall. i. red in H. des. subst.
-    exploit (UPD (ctx0 ⋅ ctx)).
-    { rewrite URA.add_assoc. et. }
-    i. des. exists (b ⋅ ctx0). split.
-    { rewrite <- URA.add_assoc. et. }
-    { exists b. uipropall. esplits; [|apply IN|refl].
-      eapply URA.add_comm. }
-  Qed.
+  (*** this is deprecated in 1.1 ***)
+  (* Lemma Own_Upd_set *)
+  (*       (r1: Σ) B *)
+  (*       (UPD: URA.updatable_set r1 B) *)
+  (*   : *)
+  (*     (Own r1) ⊢ (#=> (∃ b, ⌜B b⌝ ** (Own b))) *)
+  (* . *)
+  (* Proof. *)
+  (*   cut (Entails (Own r1) (Upd (Ex (fun b => Sepconj (Pure (B b)) (Own b))))); ss. *)
+  (*   uipropall. i. red in H. des. subst. *)
+  (*   exploit (UPD (ctx0 ⋅ ctx)). *)
+  (*   { rewrite URA.add_assoc. et. } *)
+  (*   i. des. exists (b ⋅ ctx0). split. *)
+  (*   { rewrite <- URA.add_assoc. et. } *)
+  (*   { exists b. uipropall. esplits; [|apply IN|refl]. *)
+  (*     eapply URA.add_comm. } *)
+  (* Qed. *)
 
   Lemma Own_Upd
         (r1 r2: Σ)
@@ -369,12 +363,8 @@ Section ILEMMAS.
       (Own r1) ⊢ (#=> (Own r2))
   .
   Proof.
-    iStartProof. iIntros "H".
-    iAssert (#=> (∃ b, ⌜((eq r2) b)⌝ ** (Own b)))%I with "[H]" as "H".
-    { iApply Own_Upd_set; [|iFrame].
-      red. red in UPD. i. hexploit UPD; et. }
-    iMod "H". iDestruct "H" as (b) "[#H0 H1]".
-    iPure "H0" as Hs. subst. iApply "H1".
+    uipropall. i. exists r2. esplits; et. { refl. } i. eapply UPD. eapply URA.wf_extends; et.
+    eapply URA.extends_add; et.
   Qed.
 
   Lemma Own_extends
@@ -387,44 +377,45 @@ Section ILEMMAS.
     red. uipropall. ii. etrans; et.
   Qed.
 
-  Lemma OwnM_Upd_set (M: URA.t) `{@GRA.inG M Σ}
-        (r1: M) B
-        (UPD: URA.updatable_set r1 B)
-    :
-      (OwnM r1) ⊢ (#=> (∃ b, ⌜B b⌝ ** (OwnM b)))
-  .
-  Proof.
-    assert (UPDM: URA.updatable_set
-                    (GRA.embed r1)
-                    (fun r => exists m, r = GRA.embed m /\ B m)).
-    { red. i. red in UPD.
-      unshelve hexploit UPD.
-      { eapply (@eq_rect URA.t (Σ (@GRA.inG_id _ _ H)) (@URA.car)).
-        { eapply (ctx (@GRA.inG_id _ _ H)). }
-        { symmetry. eapply (@GRA.inG_prf _ _ H). }
-      }
-      Local Transparent GRA.to_URA.
-      { ur in WF. ss. specialize (WF GRA.inG_id).
-        destruct H. subst. ss.
-        unfold GRA.embed in WF. ss.
-        replace (PeanoNat.Nat.eq_dec inG_id inG_id)
-          with (@left (inG_id = inG_id) (inG_id <> inG_id) eq_refl) in WF; ss.
-        { des_ifs. repeat f_equal. eapply proof_irrelevance. }
-      }
-      i. des. exists (GRA.embed b). esplits; et.
-      ur. Local Transparent GRA.to_URA. ss.
-      i. unfold GRA.embed. des_ifs.
-      { ss. unfold PCM.GRA.cast_ra. destruct  H. subst. ss. }
-      { ur in WF. specialize (WF k). rewrite URA.unit_idl.
-        eapply URA.wf_mon. rewrite URA.add_comm. et.
-      }
-    }
-    iIntros "H".
-    iPoseProof (Own_Upd_set with "H") as "> H".
-    { eapply UPDM. }
-    iDestruct "H" as (b) "[% H1]". des. subst.
-    iModIntro. iExists m. iFrame. ss.
-  Qed.
+  (*** this is deprecated in 1.1 ***)
+  (* Lemma OwnM_Upd_set (M: URA.t) `{@GRA.inG M Σ} *)
+  (*       (r1: M) B *)
+  (*       (UPD: URA.updatable_set r1 B) *)
+  (*   : *)
+  (*     (OwnM r1) ⊢ (#=> (∃ b, ⌜B b⌝ ** (OwnM b))) *)
+  (* . *)
+  (* Proof. *)
+  (*   assert (UPDM: URA.updatable_set *)
+  (*                   (GRA.embed r1) *)
+  (*                   (fun r => exists m, r = GRA.embed m /\ B m)). *)
+  (*   { red. i. red in UPD. *)
+  (*     unshelve hexploit UPD. *)
+  (*     { eapply (@eq_rect URA.t (Σ (@GRA.inG_id _ _ H)) (@URA.car)). *)
+  (*       { eapply (ctx (@GRA.inG_id _ _ H)). } *)
+  (*       { symmetry. eapply (@GRA.inG_prf _ _ H). } *)
+  (*     } *)
+  (*     Local Transparent GRA.to_URA. *)
+  (*     { ur in WF. ss. specialize (WF GRA.inG_id). *)
+  (*       destruct H. subst. ss. *)
+  (*       unfold GRA.embed in WF. ss. *)
+  (*       replace (PeanoNat.Nat.eq_dec inG_id inG_id) *)
+  (*         with (@left (inG_id = inG_id) (inG_id <> inG_id) eq_refl) in WF; ss. *)
+  (*       { des_ifs. repeat f_equal. eapply proof_irrelevance. } *)
+  (*     } *)
+  (*     i. des. exists (GRA.embed b). esplits; et. *)
+  (*     ur. Local Transparent GRA.to_URA. ss. *)
+  (*     i. unfold GRA.embed. des_ifs. *)
+  (*     { ss. unfold PCM.GRA.cast_ra. destruct  H. subst. ss. } *)
+  (*     { ur in WF. specialize (WF k). rewrite URA.unit_idl. *)
+  (*       eapply URA.wf_mon. rewrite URA.add_comm. et. *)
+  (*     } *)
+  (*   } *)
+  (*   iIntros "H". *)
+  (*   iPoseProof (Own_Upd_set with "H") as "> H". *)
+  (*   { eapply UPDM. } *)
+  (*   iDestruct "H" as (b) "[% H1]". des. subst. *)
+  (*   iModIntro. iExists m. iFrame. ss. *)
+  (* Qed. *)
 
   Lemma OwnM_Upd (M: URA.t) `{@GRA.inG M Σ}
         (r1 r2: M)
@@ -433,12 +424,10 @@ Section ILEMMAS.
       (OwnM r1) ⊢ (#=> (OwnM r2))
   .
   Proof.
-    iStartProof. iIntros "H".
-    iAssert (#=> (∃ b, ⌜((eq r2) b)⌝ ** (OwnM b)))%I with "[H]" as "H".
-    { iApply OwnM_Upd_set; [|iFrame].
-      red. red in UPD. i. hexploit UPD; et. }
-    iMod "H". iDestruct "H" as (b) "[#H0 H1]".
-    iPure "H0" as Hs. subst. iApply "H1".
+    uipropall. i. exists (GRA.embed r2). esplits; et.
+    { unfold OwnM in *. uipropall. refl. }
+    i. eapply GRA.embed_updatable in UPD. eapply UPD. eapply URA.wf_extends; et. eapply URA.extends_add; et.
+    unfold OwnM in H0. uipropall.
   Qed.
 
   Lemma OwnM_extends (M: URA.t) `{@GRA.inG M Σ}
